Assume functionally correct insert-after. See message.
I have spent a bunch of time trying to prove this functional
correctness, but there are a few major issues that crop up along the
way:

1. Being able to prove that if the node points to null, then insertion
   _will_ happen at the end. The issue that comes up when trying to
   prove this is that the uniqueness within a nodelist (i.e., no two
   elements in a nodelist) is a derived property, and we need this to
   be able to prove that we will always split right at the end.

2. Proving it in the "general case" (i.e., non null flink). This one
   is mostly due to the proof already being _extremely_ time consuming
   to run, that progress is taking extremely long. However, I believe
   it might be possible to factor some parts out, and push this
   functional correctness stuff into the `tot_*` functions, so as to
   (with a few choice lemmas being called) get the functional
   correctness.

3. The `lemma_split_using` within the `_l_insert_after` definition
   makes me weary.

ind/DoublyLinkedList.fst
@@ -1509,6 +1509,11 @@ let dll_insert_at_tail (#t:Type) (d:dll t) (n:pointer (node t)) :
 
 #reset-options
 
+let _l_insert_after (x0:'a) (l:list 'a{x0 `memP` l}) (x:'a) : GTot (list 'a) =
+  let l1, x1 :: l2 = lemma_split_using l x0; split_using l x0 in
+  assert (x0 == x1);
+  l1 `append` (x0 :: (x :: l2))
+
 #set-options "--z3rlimit 1000 --initial_fuel 2 --initial_ifuel 1"
 
 let dll_insert_after (#t:Type) (d:dll t) (e:pointer (node t)) (n:pointer (node t)) :
@@ -1528,7 +1533,8 @@ let dll_insert_after (#t:Type) (d:dll t) (e:pointer (node t)) (n:pointer (node t
                             (Mod.loc_buffer (e@h0).flink))) h0 h1 /\
          (dll_fp0 y `loc_equiv` B.loc_union (dll_fp0 d) (Mod.loc_buffer n)) /\
          dll_valid h1 y /\
-         unchanged_node_vals h0 h1 (reveal y.nodes))) =
+         unchanged_node_vals h0 h1 (reveal y.nodes) /\
+         reveal y.nodes == _l_insert_after e (reveal d.nodes) n)) =
   let h0 = ST.get () in
   // assert (length (reveal d.nodes) > 0);
   lemma_dll_links_contained h0 d (reveal d.nodes `index_of` e);
@@ -1536,7 +1542,9 @@ let dll_insert_after (#t:Type) (d:dll t) (e:pointer (node t)) (n:pointer (node t
   let e1 = (!*e).blink in
   let e2 = (!*e).flink in
   if is_null e2 then (
-    dll_insert_at_tail d n
+    let y = dll_insert_at_tail d n in
+    assume (reveal y.nodes == _l_insert_after e (reveal d.nodes) n);
+    y
   ) else (
     extract_nodelist_fp0 (reveal d.nodes) (reveal d.nodes `index_of` e);
     lemma_unsnoc_is_last (reveal d.nodes);
@@ -1622,6 +1630,7 @@ let dll_insert_after (#t:Type) (d:dll t) (e:pointer (node t)) (n:pointer (node t
     aux_unchanged_payload h0'' h1 e2 (reveal y.nodes);
     aux_unchanged_payload_transitive h0 h0' h0'' (reveal y.nodes);
     aux_unchanged_payload_transitive h0 h0'' h1 (reveal y.nodes);
+    assume (reveal y.nodes == _l_insert_after e (reveal d.nodes) n);
     y
   )
 
